src/ulc.lean
@@ -1,62 +1,66 @@
 -- 1. untyped lambda calculus
 
--- inductive preterm₀ : Type
--- | lam : (preterm₀ → preterm₀) → preterm₀
--- | app : preterm₀ → preterm₀ → preterm₀
+-- inductive preterm : Type
+-- | lam : (preterm → preterm) → preterm
+-- | app : preterm → preterm → preterm
 
-inductive preterm₁ (α : Type) : Type
-| var : α → preterm₁
-| lam : (α → preterm₁) → preterm₁
-| app : preterm₁ → preterm₁ → preterm₁
-open preterm₁
+inductive preterm (α : Type) : Type
+| var : α → preterm
+| lam : (α → preterm) → preterm
+| app : preterm → preterm → preterm
+open preterm
 
-def Preterm₁ : Type 1 := -- Type 1
-Π α, preterm₁ α
+def Preterm : Type 1 := -- Type 1
+Π α, preterm α
 
-def preterm₁.to_string : preterm₁ ℕ → ℕ → string
+def preterm.to_string : preterm ℕ → ℕ → string
 | (var n) _ := to_string n
-| (lam f) lv := "(λ" ++ to_string lv ++ "." ++ preterm₁.to_string (f lv) (lv + 1) ++ ")"
-| (app m₁ m₂) lv := "(" ++ preterm₁.to_string m₁ lv ++ " " ++ preterm₁.to_string m₂ lv ++ ")"
+| (lam f) lv := "(λ" ++ to_string lv ++ "." ++ preterm.to_string (f lv) (lv + 1) ++ ")"
+| (app m₁ m₂) lv := "(" ++ preterm.to_string m₁ lv ++ " " ++ preterm.to_string m₂ lv ++ ")"
 
-def Preterm₁.to_string (m : Preterm₁) : string :=
-preterm₁.to_string (m ℕ) 0
+def Preterm.to_string (m : Preterm) : string :=
+preterm.to_string (m ℕ) 0
 
-instance : has_to_string Preterm₁ :=
-⟨Preterm₁.to_string⟩
+instance : has_to_string Preterm :=
+⟨Preterm.to_string⟩
 
-def i : Preterm₁ := λ α, lam (λ x, var x)
+def i : Preterm := λ α, lam (λ x, var x)
 #eval to_string i -- "(λ0.0)"
-def s : Preterm₁ := λ α, lam (λ x, lam (λ y, lam (λ z, app (app (var x) (var z)) (app (var y) (var z)))))
+def s : Preterm := λ α, lam (λ x, lam (λ y, lam (λ z, app (app (var x) (var z)) (app (var y) (var z)))))
 #eval to_string s -- "(λ0.(λ1.(λ2.((0 2) (1 2)))))"
-def k : Preterm₁ := λ α, lam (λ x, lam (λ y, var x))
+def k : Preterm := λ α, lam (λ x, lam (λ y, var x))
 #eval to_string k -- "(λ0.(λ1.0))"
 
-def n₀ : Preterm₁ := λ α, lam (λ f, lam (λ x, var x))
+def n₀ : Preterm := λ α, lam (λ f, lam (λ x, var x))
 #eval to_string n₀  -- "(λ0.(λ1.1))"
-def n₁ : Preterm₁ := λ α, lam (λ f, lam (λ x, app (var f) (var x)))
+def n₁ : Preterm := λ α, lam (λ f, lam (λ x, app (var f) (var x)))
 #eval to_string n₁  -- "(λ0.(λ1.(0 1)))"
-def n₂ : Preterm₁ := λ α, lam (λ f, lam (λ x, app (var f) (app (var f) (var x))))
+def n₂ : Preterm := λ α, lam (λ f, lam (λ x, app (var f) (app (var f) (var x))))
 #eval to_string n₂  -- "(λ0.(λ1.(0 (0 1))))"
-def n₃ : Preterm₁ := λ α, lam (λ f, lam (λ x, app (var f) (app (var f) (app (var f) (var x)))))
+def n₃ : Preterm := λ α, lam (λ f, lam (λ x, app (var f) (app (var f) (app (var f) (var x)))))
 #eval to_string n₃  -- "(λ0.(λ1.(0 (0 (0 1)))))"
 
-def succ : Preterm₁ := λ α, lam (λ n, lam (λ f, lam (λ x, app (var f) (app (app (var n) (var f)) (var x)))))
+def succ : Preterm := λ α, lam (λ n, lam (λ f, lam (λ x, app (var f) (app (app (var n) (var f)) (var x)))))
 #eval to_string succ -- "(λ0.(λ1.(λ2.(1 ((0 1) 2)))))"
-def succ_n₀ : Preterm₁ := λ α, app (succ α) (n₀ α)
+
+def App : Preterm → Preterm → Preterm :=
+λ m₁ m₂ α, app (m₁ α) (m₂ α)
+
+def succ_n₀ : Preterm := App succ n₀
 #eval to_string succ_n₀ -- "((λ0.(λ1.(λ2.(1 ((0 1) 2))))) (λ0.(λ1.1)))"
 
-def subst' {α} : preterm₁ (preterm₁ α) → preterm₁ α
+def subst' {α} : preterm (preterm α) → preterm α
 | (var x) := x
 | (lam f) := lam (λ x, subst' (f (var x))) -- terminates!
 | (app m₁ m₂) := app (subst' m₁) (subst' m₂)
 
-def pbeta' {α} : preterm₁ (preterm₁ α) → preterm₁ α -- parallel beta
+def pbeta' {α} : preterm (preterm α) → preterm α -- parallel beta
 | (var x) := x
 | (lam f) := lam (λ x, pbeta' (f (var x)))
 | (app (lam f) m) := subst' (f (subst' m))
 | (app n m) := app (pbeta' n) (pbeta' m)
 
-def pbeta : Preterm₁ → Preterm₁ :=
+def pbeta : Preterm → Preterm :=
 λ m α, pbeta' (m _)
 
 #eval to_string succ_n₀ -- "((λ0.(λ1.(λ2.(1 ((0 1) 2))))) (λ0.(λ1.1)))"
@@ -65,7 +69,11 @@ def pbeta : Preterm₁ → Preterm₁ :=
 #eval to_string $ pbeta $ pbeta $ pbeta succ_n₀ -- "(λ0.(λ1.(0 1)))"
 #eval to_string $ pbeta $ pbeta $ pbeta $ succ_n₀ -- "(λ0.(λ1.(0 1)))"
 
-def ω : Preterm₁ := λ α, lam (λ x, app (var x) (var x))
-def Ω : Preterm₁ := λ α, app (ω α) (ω α)
+def ω : Preterm := λ α, lam (λ x, app (var x) (var x))
+def Ω : Preterm := App ω ω
 #eval to_string Ω -- "((λ0.(0 0)) (λ0.(0 0)))"
 #eval to_string $ pbeta $ Ω -- "((λ0.(0 0)) (λ0.(0 0)))"
+
+-- def isapp : Preterm₀ → Preterm₀
+-- | (lam f) := f
+-- | (app m₁ m₂) := t
